Protocols/RB/Safety.v
@@ -36,9 +36,9 @@ Proof. destruct H as (Hinit & H). hnf in H |- *. intros w Hr. induction Hr; firs
 Fact grounded_invariants : is_grounded_invariant
   (fun w => (id_coh w /\
     lift_state_inv node_state_invariants w /\
-    lift_node_inv node_psent_fwd_invariants w /\
-    lift_pkt_inv node_psent_bwd_invariants_sent w /\
-    lift_pkt_inv node_psent_bwd_invariants_recv w) /\
+    lift_node_inv node_psent_l2h_invariants w /\
+    lift_pkt_inv node_psent_h2l_invariants_sent w /\
+    lift_pkt_inv node_psent_h2l_invariants_recv w) /\
     (lift_node_inv echo_exists_before_vote w) /\
     (first_vote_due_to_echo w /\ vote_uniqueness w)).
 Proof.
@@ -54,7 +54,7 @@ Proof.
   - (* HMM proof mode? or just auto? *)
     auto using is_invariant_step_under_closed, is_invariant_step_under_split, 
       is_invariant_step_under_clear, is_invariant_step_under_intro_l, 
-      id_coh_is_invariant, state_invariants, fwd_invariants, bwd_invariants, 
+      id_coh_is_invariant, state_invariants, l2h_invariants, h2l_invariants, 
       echo_exists_before_vote_is_invariant, first_vote_due_to_echo_is_invariant, vote_uniqueness_is_invariant.
 Qed.
 
@@ -65,15 +65,15 @@ Ltac saturate :=
   let Htmp := fresh "Htmp" in
   let Hcoh := fresh "Hcoh" in
   let Hst := fresh "Hst" in
-  let Hfwd := fresh "Hfwd" in
-  let Hbwds := fresh "Hbwds" in
-  let Hbwdr := fresh "Hbwdr" in
+  let Hl2h := fresh "Hl2h" in
+  let Hh2ls := fresh "Hh2ls" in
+  let Hh2lr := fresh "Hh2lr" in
   let Heebr := fresh "Heebr" in
   let Hvu := fresh "Hvu" in
   match goal with
     H : reachable ?w |- _ => 
     pose proof (grounded_invariant_is_safety grounded_invariants) as Htmp; specialize (Htmp _ H);
-    simpl in Htmp; destruct Htmp as ((Hcoh & Hst & Hfwd & Hbwds & Hbwdr) & Heebr & (_ (* not useful here *) & Hvu))
+    simpl in Htmp; destruct Htmp as ((Hcoh & Hst & Hl2h & Hh2ls & Hh2lr) & Heebr & (_ (* not useful here *) & Hvu))
   end.
 
 Definition vote_integrity w : Prop :=
@@ -109,23 +109,23 @@ Proof.
   hnf. intros w Hr. saturate.
   hnf. intros dst src r v Hnonbyz_dst Hnonbyz_src H2.
   apply Heebr (* also a step *) in H2; auto. hnf in H2. saturate_assumptions. destruct H2 as (src' & dst' & Hnonbyz_src' & Hin'').
-  pick echomsg_sent_bwd as_ H3 by_ (pose proof (Hbwds _ Hin'') as []). saturate_assumptions.
-  pick initialmsg_recv_fwd as_ H4 by_ (pose proof (Hfwd _ Hnonbyz_src') as []). specialize (H4 _ _ _ H3). rewrite Hcoh in H4.
-  pick initialmsg_sent_bwd as_ H5 by_ (pose proof (Hbwds _ H4) as []). now saturate_assumptions.
+  pick echomsg_sent_h2l as_ H3 by_ (pose proof (Hh2ls _ Hin'') as []). saturate_assumptions.
+  pick initialmsg_recv_l2h as_ H4 by_ (pose proof (Hl2h _ Hnonbyz_src') as []). specialize (H4 _ _ _ H3). rewrite Hcoh in H4.
+  pick initialmsg_sent_h2l as_ H5 by_ (pose proof (Hh2ls _ H4) as []). now saturate_assumptions.
 Qed.
 
 Lemma output_integrity_is_safety : is_safety output_integrity.
 Proof.
   hnf. intros w Hr. saturate.
   hnf. intros dst src r v Hnonbyz_dst Hnonbyz_src Hin.
-  pick output_coh_fwd as_ H1 by_ (pose proof (Hst dst) as []). specialize (H1 _ _ _ Hin). 
+  pick output_vote_size as_ H1 by_ (pose proof (Hst dst) as []). specialize (H1 _ _ _ Hin). 
   (* TODO the following two steps have some overlap with a previous proof *)
   unfold th_vote4output in H1. pose proof t0_lt_N_minus_2t0 as Ht0.
-  pick msgcnt_coh as_ Hnodup by_ (pose proof (Hst dst) as []). 
+  pick msgcnt_nodup as_ Hnodup by_ (pose proof (Hst dst) as []). 
   match type of H1 with _ <= ?ll => assert (t0 < ll) as (n & Hnonbyz_n & Hin')%at_least_one_nonfaulty by lia end.
   2: eapply (Hnodup (VoteMsg _ _ _)).
-  pick msgcnt_recv_fwd as_ H2 by_ (pose proof (Hfwd _ Hnonbyz_dst) as []). specialize (H2 _ _ Hin'). rewrite Hcoh in H2.
-  pick votemsg_sent_bwd as_ H4 by_ (pose proof (Hbwds _ H2) as []). saturate_assumptions.
+  pick msgcnt_recv_l2h as_ H2 by_ (pose proof (Hl2h _ Hnonbyz_dst) as []). specialize (H2 _ _ Hin'). rewrite Hcoh in H2.
+  pick votemsg_sent_h2l as_ H4 by_ (pose proof (Hh2ls _ H2) as []). saturate_assumptions.
   (* use vote_integrity *)
   apply vote_integrity_is_safety in Hr. apply Hr in H4; auto.
 Qed.
@@ -135,23 +135,23 @@ Proof.
   hnf. intros w Hr. saturate.
   hnf. intros dst1 dst2 src r v1 v2 Hnonbyz_dst1 Hnonbyz_dst2 Hin1 Hin2.
   destruct (Value_eqdec v1 v2) as [ | Hneq ]; auto.
-  pick output_coh_fwd as_ Hle1 by_ (pose proof (Hst dst1) as []). specialize (Hle1 _ _ _ Hin1).
-  pick output_coh_fwd as_ Hle2 by_ (pose proof (Hst dst2) as []). specialize (Hle2 _ _ _ Hin2). 
+  pick output_vote_size as_ Hle1 by_ (pose proof (Hst dst1) as []). specialize (Hle1 _ _ _ Hin1).
+  pick output_vote_size as_ Hle2 by_ (pose proof (Hst dst2) as []). specialize (Hle2 _ _ _ Hin2). 
   (* TODO the following step has some overlap with a previous proof *)
   unfold th_vote4output in Hle1, Hle2.
-  pick msgcnt_coh as_ Hnodup1 by_ (pose proof (Hst dst1) as []). specialize (Hnodup1 (VoteMsg src r v1)).
-  pick msgcnt_coh as_ Hnodup2 by_ (pose proof (Hst dst2) as []). specialize (Hnodup2 (VoteMsg src r v2)).
+  pick msgcnt_nodup as_ Hnodup1 by_ (pose proof (Hst dst1) as []). specialize (Hnodup1 (VoteMsg src r v1)).
+  pick msgcnt_nodup as_ Hnodup2 by_ (pose proof (Hst dst2) as []). specialize (Hnodup2 (VoteMsg src r v2)).
   simpl in Hnodup1, Hnodup2.
   (* the basic idea is to find a non-faulty node in the quorum intersection that equivocate, and then prove False *)
   pose proof (quorum_intersection Hnodup1 Hnodup2 Hle1 Hle2) as Hq. pose proof t0_lt_N_minus_2t0 as Ht0.
   match type of Hq with _ <= ?ll => assert (t0 < ll) as (n & Hnonbyz_n & (Hin2' & Hin1'%in_dec_is_left)%filter_In)%at_least_one_nonfaulty by lia end.
   2: now apply List.NoDup_filter.
   (* TODO the following step has some overlap with a previous proof *)
-  pick msgcnt_recv_fwd as_ Hsent1 by_ (pose proof (Hfwd _ Hnonbyz_dst1) as []). specialize (Hsent1 _ _ Hin1'). 
-  pick msgcnt_recv_fwd as_ Hsent2 by_ (pose proof (Hfwd _ Hnonbyz_dst2) as []). specialize (Hsent2 _ _ Hin2').
+  pick msgcnt_recv_l2h as_ Hsent1 by_ (pose proof (Hl2h _ Hnonbyz_dst1) as []). specialize (Hsent1 _ _ Hin1'). 
+  pick msgcnt_recv_l2h as_ Hsent2 by_ (pose proof (Hl2h _ Hnonbyz_dst2) as []). specialize (Hsent2 _ _ Hin2').
   rewrite Hcoh in Hsent1, Hsent2.
-  pick votemsg_sent_bwd as_ Hv1 by_ (pose proof (Hbwds _ Hsent1) as []).
-  pick votemsg_sent_bwd as_ Hv2 by_ (pose proof (Hbwds _ Hsent2) as []).
+  pick votemsg_sent_h2l as_ Hv1 by_ (pose proof (Hh2ls _ Hsent1) as []).
+  pick votemsg_sent_h2l as_ Hv2 by_ (pose proof (Hh2ls _ Hsent2) as []).
   saturate_assumptions. congruence.
 Qed.
 
@@ -164,7 +164,7 @@ Proof.
   (* by using uniqueness_is_safety and setting dst1 = dst2 = dst *)
   pose proof (output_uniqueness_is_safety Hr src r x y Hnonbyz_dst Hnonbyz_dst
     ltac:(rewrite <- E; simpl; tauto) ltac:(rewrite <- E; simpl; tauto)) as ->.
-  pick output_coh as_ Hnodup by_ (pose proof (Hst dst) as []). specialize (Hnodup src r). 
+  pick output_nodup as_ Hnodup by_ (pose proof (Hst dst) as []). specialize (Hnodup src r). 
   rewrite <- E, -> ! NoDup_cons_iff in Hnodup. simpl in Hnodup. tauto.
 Qed.
 
